codelib/CodeLib.lean
@@ -77,6 +77,7 @@ import CodeLib.SepLogic.SmallStepOutcomeExample
 import CodeLib.SepLogic.SmallStepAdequacy
 import CodeLib.SepLogic.SmallStepAdequacyExamples
 import CodeLib.SepLogic.SmallStepOutcomeAdequacy
+import CodeLib.SepLogic.SmallStepOutcomeAdequacyFrontier
 import CodeLib.Examples.MergeSort.TotalProof
 import CodeLib.Examples.Quicksort.TotalProof
 import CodeLib.Examples.SelectionSort.StdIOProof
